@prefix ponto: <http://www.mobr.ai/ontologies/ponto#> .
@prefix owl: <http://www.w3.org/2002/07/owl#> .
@prefix rdf: <http://www.w3.org/1999/02/22-rdf-syntax-ns#> .
@prefix rdfs: <http://www.w3.org/2000/01/rdf-schema#> .
@prefix dc: <http://purl.org/dc/elements/1.1/> .
@prefix dcterms: <http://purl.org/dc/terms/> .
@prefix ns: <http://www.w3.org/2003/06/sw-vocab-status/ns#> .
@prefix vann: <http://purl.org/vocab/vann/> .
@prefix xml: <http://www.w3.org/XML/1998/namespace> .
@prefix xsd: <http://www.w3.org/2001/XMLSchema#> .
@base <http://www.mobr.ai/ontologies/ponto#> .

<http://www.mobr.ai/ontologies/ponto#> rdf:type owl:Ontology .

<http://www.mobr.ai/ontologies/ponto#> a owl:Ontology ;
	owl:versionIRI <http://www.mobr.ai/ontologies/ponto/v0/> ;
	owl:imports <http://www.w3.org/2003/06/sw-vocab-status/ns> ;
	dc:contributor "Marcio Moreno" , "Rafael Brandao" ;
	dc:creator "MOBR Systems" ;
	dc:title "POnto - An ontology for the Polkadot ecosystem" ;
	vann:preferredNamespacePrefix "ponto" ;
	rdfs:comment "This Polkadot ontology specification uses W3C RDF Schema and the Web Ontology Language. Its main source of information comes from the Polkadot Whitepaper written by Dr. Gavin Wood."@en ;
	rdfs:seeAlso <https://github.com/mobr-ai/POnto> , <https://polkadot.network/whitepaper/> ;
	owl:versionInfo "0.1" ;
	ns:term_status "unstable" ;
    dc:license <https://www.apache.org/licenses/LICENSE-2.0> .

<https://www.apache.org/licenses/LICENSE-2.0>
    rdf:type dcterms:LicenseDocument ;
    dc:title "Apache License, Version 2.0" .

# this ontology uses modules aiming at a better organization
<http://www.mobr.ai/ontologies/ponto/consensus#> rdf:type owl:Ontology .
<http://www.mobr.ai/ontologies/ponto/consensus#> owl:imports <Consensus.ttl> .

<http://www.mobr.ai/ontologies/ponto/governance#> rdf:type owl:Ontology .
<http://www.mobr.ai/ontologies/ponto/governance#> owl:imports <Governance.ttl> .

<http://www.mobr.ai/ontologies/ponto/ledger#> rdf:type owl:Ontology .
<http://www.mobr.ai/ontologies/ponto/ledger#> owl:imports <Ledger.ttl> .

<http://www.mobr.ai/ontologies/ponto/Oracle#> rdf:type owl:Ontology .
<http://www.mobr.ai/ontologies/ponto/Oracle#> owl:imports <Oracle.ttl> .

<http://www.mobr.ai/ontologies/ponto/RBox#> rdf:type owl:Ontology .
<http://www.mobr.ai/ontologies/ponto/RBox#> owl:imports <RBox.ttl> .

<http://www.mobr.ai/ontologies/ponto/Stake#> rdf:type owl:Ontology .
<http://www.mobr.ai/ontologies/ponto/Stake#> owl:imports <Stake.ttl> .

<http://www.mobr.ai/ontologies/ponto/Token#> rdf:type owl:Ontology .
<http://www.mobr.ai/ontologies/ponto/Token#> owl:imports <Token.ttl> .

<http://www.mobr.ai/ontologies/ponto/Tooling#> rdf:type owl:Ontology .
<http://www.mobr.ai/ontologies/ponto/Tooling#> owl:imports <Tooling.ttl> .

<http://www.mobr.ai/ontologies/ponto/Transaction#> rdf:type owl:Ontology .
<http://www.mobr.ai/ontologies/ponto/Transaction#> owl:imports <Transaction.ttl> .

<http://www.mobr.ai/ontologies/ponto/Wallet#> rdf:type owl:Ontology .
<http://www.mobr.ai/ontologies/ponto/Wallet#> owl:imports <Wallet.ttl> .


# basic ontology definitions

# general notion: a system architecture is composed by a group of components.

ponto:Architecture a owl:Class ;
    rdfs:label "System Architecture" ;
    rdfs:comment "A high-level structure of a software system that defines its components, their relationships, and their interactions." ;
    rdfs:subClassOf owl:Thing .

ponto:Component a owl:Class ;
    rdfs:label "Architecture Component" ;
    rdfs:comment "A specific technology component that composes ledger architecture or implementation." ;
    rdfs:subClassOf owl:Thing .

# A component is a part of an architecture
ponto:partOf rdf:type rdf:Property ;
    rdfs:domain ponto:Component ;
    rdfs:range ponto:Architecture .

# An architecture is composed of components
ponto:hasComponent rdf:type rdf:Property ;
    rdfs:domain ponto:Architecture ;
    rdfs:range ponto:Component .


# ledger basic definitions

ponto:LedgerArchitecture a owl:Class ;
    rdfs:label "Ledger Architecture" ;
    rdfs:comment "A specific design and organization of components that make up a distributed and decentralized ledger system. It defines the rules and protocols for how different parts of the system interact with each other to achieve the desired functionality and security." ;
    rdfs:subClassOf ponto:Architecture .

ponto:LedgerRecord a owl:Class ;
    rdfs:label "Ledger Record" ;
    rdfs:comment "A digital record that contains information about a specific event or transaction that has occurred on the blockchain." ;
    rdfs:subClassOf ponto:Component .

ponto:DistributedLedger a owl:Class ;
    rdfs:label "Distributed Ledger" ;
    rdfs:comment "A decentralized and distributed digital ledger that is maintained by a network of computers (nodes) that participate in the network." ;
    rdfs:subClassOf ponto:Component .

ponto:SmartContractPlatform a owl:Class ;
    rdfs:label "Smart Contract Platform" ;
    rdfs:comment "A software platform that enables the deployment and execution of smart contracts on the Polkadot network." ;
    rdfs:subClassOf ponto:Component .

ponto:PolkadotArchitecture a owl:Class ;
    rdfs:label "Polkadot Architecture" ;
    rdfs:comment "An architecture based on a multichain network that includes several different types of chains, each with its own specific purpose and functionality. The core of the architecture is a relay chain that facilitates communication with parachains and parathreads." ;
    rdfs:subClassOf ponto:LedgerArchitecture .

ponto:RelayChain a owl:Class ;
    rdfs:label "Relay Chain" ;
    rdfs:comment "The main chain in the Polkadot ecosystem that coordinates communication between parachains. The Relay Chain is the central hub of the Polkadot network, which coordinates and connects all the parachains in the ecosystem." ;
    rdfs:subClassOf ponto:Component .

ponto:Parachain a owl:Class ;
    rdfs:label "Parachain" ;
    rdfs:comment "An independent blockchain that connects and relies on the Polkadot Relay Chain for security and interoperability purposes." ;
    rdfs:subClassOf ponto:Component .

ponto:Parathread a owl:Class ;
    rdfs:label "Parathread" ;
    rdfs:comment "A type of parachain that allows for dynamic participation and payment for security." ;
    rdfs:subClassOf ponto:Parachain ;
    rdfs:partOf ponto:PolkadotArchitecture .

ponto:Bridge a owl:Class ;
    rdfs:label "Bridge" ;
    rdfs:comment "A mechanism for connecting external blockchains to the Polkadot ecosystem." ;
    rdfs:subClassOf ponto:Component ;
    rdfs:partOf ponto:Parachain .

ponto:Wallet a owl:Class ;
    rdfs:label "Wallet" ;
    rdfs:comment "A software application that stores private keys and allows users to manage their cryptocurrencies." ;
    rdfs:subClassOf ponto:Component .

# Classes for Polkadot nodes
ponto:Node a owl:Class ;
    rdfs:label "Node" ;
    rdfs:comment "A component that participates in the Polkadot network." ;
    rdfs:subClassOf ponto:Component .

ponto:FullNode a owl:Class ;
    rdfs:label "Full Node" ;
    rdfs:comment "A node that stores a full copy of the blockchain and participates in block validation." ;
    rdfs:subClassOf ponto:Node .

ponto:LightNode a owl:Class ;
    rdfs:label "Light Node" ;
    rdfs:comment "A node that only stores a subset of the blockchain data and relies on other nodes for information." ;
    rdfs:subClassOf ponto:Node .

# in the polkadot ecosystem, a validator can operate as either full nodes or as light nodes, depending on its resources and network requirements.
ponto:Validator a owl:Class ;
    rdfs:label "Validator" ;
    rdfs:comment "A node responsible for validating transactions and blocks." ;
    rdfs:subClassOf ponto:Node .

# in the polkadot ecosystem, a collator is desirably a full nodes, but it is not a requirement.
ponto:Collator a owl:Class ;
    rdfs:label "Collator" ;
    rdfs:comment "A node on a parachain that is responsible for responsible for collecting transactions and building new blocks. While they communicate with the Relay Chain, they are not on the Relay Chain themselves." ;
    rdfs:subClassOf ponto:Node ;
    rdfs:partOf ponto:Parachain .

# person or organization
ponto:AccountHolder a owl:Class ;
    rdfs:label "Account Holder" ;
    rdfs:comment "An entity that holds one or more accounts, such as an individual or organization." ;
    rdfs:subClassOf owl:Thing .

# Defining Relationships

# A ledger implements an architecture
ponto:implements rdf:type rdf:Property ;
    rdfs:domain ponto:LedgerArchitecture ;
    rdfs:range ponto:DistributedLedger .

# parachain
# A parachain is part of polkadot architecture
ponto:partOf rdf:type rdf:Property ;
    rdfs:domain ponto:Parachain ;
    rdfs:range ponto:PolkadotArchitecture .

# A polkadot architecture has parachain
ponto:hasParachain rdf:type rdf:Property ;
    rdfs:domain ponto:PolkadotArchitecture ;
    rdfs:range ponto:Parachain .


# relay chain
# A relay chain is part of polkadot architecture
ponto:partOf rdf:type rdf:Property ;
    rdfs:domain ponto:RelayChain ;
    rdfs:range ponto:PolkadotArchitecture .

# A polkadot architecture has relay chain
ponto:hasParachain rdf:type rdf:Property ;
    rdfs:domain ponto:PolkadotArchitecture ;
    rdfs:range ponto:RelayChain .


# bridge
ponto:usesBridge rdfs:domain ponto:RelayChain ;
    rdfs:range ponto:Bridge .

ponto:usesBridge rdfs:domain ponto:Parachain ;
    rdfs:range ponto:Bridge .

ponto:usesBridge ponto:DisjointClasses [
    owl:members (
        ponto:Parachain
        ponto:RelayChain
    )
] .
