@prefix ponto: <http://www.mobr.ai/ontologies/ponto#> .
@prefix owl: <http://www.w3.org/2002/07/owl#> .
@prefix rdf: <http://www.w3.org/1999/02/22-rdf-syntax-ns#> .
@prefix rdfs: <http://www.w3.org/2000/01/rdf-schema#> .

# smart contract platforms and other toolings in the Polkadot Ecosystem

ponto:Substrate a owl:Class ;
    rdfs:label "Substrate" ;
    rdfs:comment "A blockchain development framework that provides provides a set of tools and libraries that developers can use to build customized blockchain networks and smart contract platforms." ;
    rdfs:subClassOf ponto:SmartContractPlatform .

ponto:Ink a owl:Class ;
    rdfs:label "Ink!" ;
    rdfs:comment "a high-level programming language designed specifically for writing smart contracts on the Polkadot network." ;
    rdfs:subClassOf ponto:SmartContractPlatform .

ponto:PSCR a owl:Class ;
    rdfs:label "Parity Smart Contract Runtime" ;
    rdfs:comment "A lightweight, modular runtime environment for executing smart contracts on the Polkadot network." ;
    rdfs:subClassOf ponto:SmartContractPlatform .

ponto:Wasm a owl:Class ;
    rdfs:label "WebAssembly" ;
    rdfs:comment "A low-level virtual machine that is used to run smart contracts on Polkadot." ;
    rdfs:subClassOf ponto:Component .

ponto:PolkadotJS a owl:Class ;
    rdfs:label "Polkadot JS" ;
    rdfs:comment "A collection of libraries and tools for building Polkadot applications in JavaScript." ;
    rdfs:subClassOf ponto:Component .
