@prefix ponto: <http://www.mobr.ai/ontologies/ponto#> .
@prefix owl: <http://www.w3.org/2002/07/owl#> .
@prefix rdf: <http://www.w3.org/1999/02/22-rdf-syntax-ns#> .
@prefix rdfs: <http://www.w3.org/2000/01/rdf-schema#> .

# transactions in the Polkadot Ecosystem

ponto:Transaction a rdfs:Class ;
    rdfs:label "Transaction" ;
    rdfs:comment "A transaction in the Polkadot blockchain, representing the transfer of assets between two parties." ;
    rdfs:subClassOf ponto:LedgerRecord .

ponto:Sender a rdfs:Class ;
    rdfs:label "Sender" ;
    rdfs:comment "The entity sending assets in a Polkadot blockchain transaction." ;
    rdfs:subClassOf ponto:Account .

ponto:Recipient a rdfs:Class ;
    rdfs:label "Recipient" ;
    rdfs:comment "The entity receiving assets in a Polkadot blockchain transaction." ;
    rdfs:subClassOf ponto:Account .

# properties
ponto:amountTransferred a owl:DatatypeProperty ;
    rdfs:comment "The amount of assets transferred in a Polkadot blockchain transaction." ;
    rdfs:domain ponto:Transaction ;
    rdfs:range xsd:decimal .

ponto:typeOfAsset a owl:DatatypeProperty ;
    rdfs:comment "The type of asset transferred in a Polkadot blockchain transaction." ;
    rdfs:domain ponto:Transaction ;
    rdfs:range xsd:string .

ponto:uniqueID a owl:DatatypeProperty ;
    rdfs:comment "The unique identification number of a record in the Polkadot blockchain." ;
    rdfs:domain ponto:Record ;
    rdfs:range xsd:string .

ponto:hasRecord a owl:ObjectProperty ;
    rdfs:comment "The record associated with a Polkadot blockchain transaction." ;
    rdfs:domain ponto:Transaction ;
    rdfs:range ponto:Record .

ponto:hasSender a owl:ObjectProperty ;
    rdfs:comment "The sender of a Polkadot blockchain transaction." ;
    rdfs:domain ponto:Transaction ;
    rdfs:range ponto:Sender .

ponto:hasRecipient a owl:ObjectProperty ;
    rdfs:comment "The recipient of a Polkadot blockchain transaction." ;
    rdfs:domain ponto:Transaction ;
    rdfs:range ponto:Recipient .

ponto:belongsToBlock a owl:ObjectProperty ;
    rdfs:comment "The block where the transaction is recorded" ;
    rdfs:domain ponto:Transaction ;
    rdfs:range ponto:Block .
