@prefix ponto: <http://www.mobr.ai/ontologies/ponto#> .
@prefix owl: <http://www.w3.org/2002/07/owl#> .
@prefix rdf: <http://www.w3.org/1999/02/22-rdf-syntax-ns#> .
@prefix rdfs: <http://www.w3.org/2000/01/rdf-schema#> .

# consensus mechanisms in the Polkadot Ecosystem
ponto:FinalityGadget a owl:Class ;
    rdfs:label "Finality Gadget" ;
    rdfs:comment "A mechanism that determines finality." ;
    rdfs:subClassOf ponto:Component .

ponto:ConsensusMechanism a owl:Class ;
    rdfs:label "Consensus Mechanism" ;
    rdfs:comment "The mechanism by which nodes on a distributed ledger agree on a set of valid transactions and blocks." ;
    rdfs:subClassOf ponto:FinalityGadget .

ponto:ProofOfWork a owl:Class ;
    rdfs:label "Proof of Work" ;
    rdfs:comment "A method of selecting participants in a consensus system, typically the longest chain rule, in which participants try to solve a puzzle like finding a partial pre-image of a hash. Normally, a Proof-of-Work system can have any number of participants." ;
    rdfs:subClassOf ponto:ConsensusMechanism .

ponto:ProofOfStake a owl:Class ;
    rdfs:label "Proof of Stake" ;
    rdfs:comment "A method of selecting participation in a consensus system, in which participants are chosen based on how many tokens they have at stake (at risk of loss due to misbehavior). Normally, Proof-of-Stake systems limit the number of participants." ;
    rdfs:subClassOf ponto:ConsensusMechanism .

ponto:NPoS a owl:Class ;
    rdfs:label "Nominated Proof of Stake" ;
    rdfs:comment "A Proof-of-Stake system where nominators back validators with their own stake as a show of faith in the good behavior of the validator. Nominated Proof-of-Stake differs from the more generic concept Delegated Proof-of-Stake in that nominators are subject to loss of stake if they nominate a bad validator; delegators are not subject to loss of stake based on the behavior of the validator. Note that some other blockchain technologies may use the term Delegated Proof-of-Stake, even if delegators can be slashed. Polkadot uses the Phragm√©n method to allocate stake to nominees." ;
    rdfs:subClassOf ponto:ProofOfStake .

ponto:Grandpa a owl:Class ;
    rdfs:label "GRANDPA" ;
    rdfs:comment "GRANDPA (GHOST-based Recursive Ancestor Deriving Prefix Agreement) is a proof-of-stake consensus mechanism used in the Polkadot ecosystem." ;
    rdfs:subClassOf ponto:ProofOfStake .

ponto:Finality a owl:Class ;
    rdfs:label "Finality" ;
    rdfs:comment "The property of a block that cannot be reverted. Generally, created blocks are not final until some point in the future - perhaps never, in the case of 'probabilistic finality'. The Polkadot Relay Chain uses a deterministic finality gadget known as GRANDPA." ;
    rdfs:subClassOf owl:Thing .

ponto:Safety a owl:Class ;
    rdfs:label "Safety" ;
    rdfs:comment "The property of a distributed system indicating that a particular state transition will not be reverted. GRANDPA provides deterministic safety. That is, for a state changed marked as 'safe' or 'final', one would require a hard fork to revert that change." ;
    rdfs:subClassOf owl:Thing .

ponto:Session a owl:Class ;
    rdfs:label "Session" ;
    rdfs:comment "A session is a Substrate implementation term for a period that has a constant set of validators. Validators can only join or exit the validator set at a session change." ;
    rdfs:subClassOf owl:Thing .

ponto:Slashing a owl:Class ;
    rdfs:label "Slashing" ;
    rdfs:comment "The removal of a percentage of an account's DOT as a punishment for a validator acting maliciously or incompetently (e.g., equivocating or remaining offline for an extended period)." ;
    rdfs:subClassOf owl:Thing .

ponto:Nominator a owl:Class ;
    rdfs:label "Nominator" ;
    rdfs:comment "Accounts that select a set of validators to nominate by bonding their tokens. Nominators receive some of the validators' rewards, but are also liable for slashing if their nominated validators misbehave." ;
    rdfs:subClassOf ponto:StakeHolder .

ponto:Era a owl:Class ;
    rdfs:label "Era" ;
    rdfs:comment "A (whole) number of sessions, which is the period that the validator set (and each validator's active nominator set) is recalculated and where rewards are paid out." ;
    rdfs:subClassOf ponto:Component .

ponto:ActiveNomination a owl:Class ;
    rdfs:label "Active Nomination" ;
    rdfs:comment "A validator (or validators) that a nominator has selected to nominate and is actively validating this era. The nominator is placing their stake behind this validator for this era and will potentially receive staking rewards in return for doing so." ;
    rdfs:subClassOf ponto:Validator .

ponto:InactiveNomination a owl:Class ;
    rdfs:label "Inactive Nomination" ;
    rdfs:comment "A validator (or validators) that a nominator has selected to nominate, but is not actively validating this era. This type of nomination may become active in a future era." ;
    rdfs:subClassOf ponto:Validator .

ponto:Attestation a owl:Class ;
    rdfs:label "Era" ;
    rdfs:comment "A type of message that validators broadcast that says whether they think a parachain candidate block is valid or invalid." ;
    rdfs:subClassOf ponto:Component .

ponto:Authority a owl:Class ;
    rdfs:label "Authority" ;
    rdfs:comment "A generic term for the role in a blockchain that can participate in the consensus mechanisms. In GRANDPA, the authorities vote on chains they consider final. In BABE, the authorities are block producers. Authority sets can be chosen to be mechanisms such as Polkadot's NPoS algorithm." ;
    rdfs:subClassOf ponto:Component .

ponto:Babe a owl:Class ;
    rdfs:label "BABE" ;
    rdfs:comment "Blind Assignment for Blockchain Extension (BABE) is the Polkadot's block production mechanism." ;
    rdfs:subClassOf ponto:Component .

ponto:BLS a owl:Class ;
    rdfs:label "BLS" ;
    rdfs:comment "Boneh-Lynn-Shacham (BLS) is a signature scheme for voting in consensus algorithms and threshold signatures. BLS signatures have a slow signing, very slow verification, require slow and much less secure pairing friendly curves, and tend towards dangerous malleability. Yet, BLS permits a diverse array of signature aggregation options far beyond any other known signature scheme, which makes BLS a preferred scheme for voting in consensus algorithms and threshold signatures." ;
    rdfs:subClassOf ponto:Component .

ponto:Candidate a owl:Class ;
    rdfs:label "Candidate" ;
    rdfs:comment "Is a submitted parachain block to the relay chain validators. A parachain block stops being referred to as a candidate as soon it has been finalized." ;
    rdfs:subClassOf ponto:Block .

ponto:Collations a owl:Class ;
    rdfs:label "Collations" ;
    rdfs:comment "Parachain blocks or candidates that are being proposed to the Polkadot relay chain validators. More specifically, a collation is a data structure which contains the proposed parachain candidate, including an optional validation parachain Runtime update and upward messages." ;
    rdfs:subClassOf ponto:Candidate .

ponto:Commission a owl:Class ;
    rdfs:label "Commission" ;
    rdfs:comment "Determines the rate of distribution for the remaining rewards set out for the nominators that are backing that validator." ;
    rdfs:subClassOf ponto:Component .

ponto:DutyRoster a owl:Class ;
    rdfs:label "Duty Roster" ;
    rdfs:comment "A lookup table that specifies the job that a particular validator is required to do (i.e. attest to the validity of a specific parachain). The duty roster routinely shuffles the validator set into different subsets per parachain." ;
    rdfs:subClassOf ponto:Component .

ponto:Epoch a owl:Class ;
    rdfs:label "Epoch" ;
    rdfs:comment "An epoch is a time duration in the BABE protocol that is broken into smaller time slots." ;
    rdfs:subClassOf ponto:Component .

ponto:EpochTimeSlot a owl:Class ;
    rdfs:label "Epoch Time Slot" ;
    rdfs:comment "A time slot that compose an epoch." ;
    rdfs:subClassOf ponto:Component .

ponto:SlotLeader a owl:Class ;
    rdfs:label "Slot Leader" ;
    rdfs:comment "Each time slot that compose an epoch has at least one slot leader who has the right to propose a block." ;
    rdfs:subClassOf ponto:Component .

ponto:Equivocation a owl:Class ;
    rdfs:label "Equivocation" ;
    rdfs:comment "Providing conflicting information to the network. BABE equivocation entails creating multiple blocks in the same slot. GRANDPA equivocation would consist of signing multiple conflicting chains." ;
    rdfs:subClassOf owl:Thing .

ponto:Liveness a owl:Class ;
    rdfs:label "Liveness" ;
    rdfs:comment "The property of a distributed system is that it will eventually come to some sort of consensus. A system stuck in an infinite loop would not be considered live, even if computations are taking place; a system that eventually provides a result, even if incorrect or it takes a long time, is considered to have liveness." ;
    rdfs:subClassOf owl:Thing .

ponto:NextSession a owl:Class ;
    rdfs:label "Next Session" ;
    rdfs:comment "This indicates that the validator will be a member of the active set in the next session." ;
    rdfs:subClassOf owl:Thing .

ponto:OnlineMessage a owl:Class ;
    rdfs:label "Online Message" ;
    rdfs:comment "This is a message that is broadcast by a validator to verify to the network that the validator is online, even if they haven't published a block this epoch. This is sometimes referred to as 'ImOnline'." ;
    rdfs:subClassOf owl:Thing .

ponto:Oversubscribed a owl:Class ;
    rdfs:label "Oversubscribed" ;
    rdfs:comment "If more than the maximum number of nominators nominate the same validator, it is 'oversubscribed', and only the top staked nominators (ranked by the amount of stake, up to the maximum number of nominators) are paid rewards. Other nominators will receive no rewards for that era. The current maximum number of nominators is 512 on Polkadot, but it can be modified via governance." ;
    rdfs:subClassOf owl:Thing .

ponto:Preimage a owl:Class ;
    rdfs:label "Preimage" ;
    rdfs:comment "The on-chain proposals do not require the entire image of extrinsics and data (for instance the WASM code, in case of upgrades) to be submitted, but would rather just need that image's hash. That preimage can be submitted and stored on-chain against the hash later, upon the proposal's dispatch." ;
    rdfs:subClassOf owl:Thing .

ponto:ProofOfValidity a owl:Class ;
    rdfs:label "Proof of Validity" ;
    rdfs:comment "A proof produced by parachain collators. Based on this proof and the parachain registry, a validator can verify that a parachain has properly executed its state transition function. Proofs of Validity go into the Relay Chain blocks." ;
    rdfs:subClassOf owl:Thing .

ponto:RandomSeed a owl:Class ;
    rdfs:label "Random Seed" ;
    rdfs:comment "A random seed is a pseudo-random number available on-chain. It is used in various places of the Polkadot protocol, most prominently in BABE the block production mechanism." ;
    rdfs:subClassOf owl:Thing .

# literals
ponto:capacity a xsd:integer ;
    rdfs:label "capacity" ;
    rdfs:comment "The maximum number of nominators signalling intent to nominate a validator (and thus could potentially actively nominate that validator in the next session). This maximum number will equal the number of nominators necessary to oversubscribe a validator. Any validator which is 'at capacity' or higher may potentially be oversubscribed in the next session; a validator that is not at capacity cannot be oversubscribed unless more nominators select it before the next election." .

# relationships
ponto:producesProof a rdf:Property ;
    rdfs:domain ponto:Collator ;
    rdfs:range ponto:ProofOfValidity .

ponto:hasTimeSlot a rdf:Property ;
    rdfs:domain ponto:Epoch ;
    rdfs:range xsd:EpochTimeSlot .

ponto:hasSlotLeader a rdf:Property ;
    rdfs:domain ponto:EpochTimeSlot ;
    rdfs:range xsd:SlotLeader .

ponto:blocksNomination a rdf:Property ;
    rdfs:label "blocks nomination" ;
    rdfs:comment "Indicates that a validator does not currently allow any more nominations. This is controlled by the validator." ;
    rdfs:domain ponto:Validator ;
    rdfs:range xsd:boolean .

ponto:hasDuty a rdf:Property ;
    rdfs:domain ponto:Validator ;
    rdfs:range xsd:DutyRoster .

ponto:validatorAtCapacity a owl:ObjectProperty ;
    rdfs:comment "The maximum number of nominators signalling intent to nominate a validator (and thus could potentially actively nominate that validator in the next session). This maximum number will equal the number of nominators necessary to oversubscribe a validator. Any validator which is 'at capacity' or higher may potentially be oversubscribed in the next session; a validator that is not at capacity cannot be oversubscribed unless more nominators select it before the next election." ;
    rdfs:domain ponto:Validator ;
    rdfs:range ponto:capacity .

ponto:hasValidator a owl:ObjectProperty ;
    rdfs:domain ponto:Collator ;
    rdfs:range ponto:Validator .

ponto:hasNominator a owl:ObjectProperty ;
    rdfs:domain ponto:StakeHolder ;
    rdfs:range ponto:Nominator .

ponto:proposesBlock a owl:ObjectProperty ;
    rdfs:domain ponto:Validator ;
    rdfs:range ponto:Transaction ;
    rdfs:comment "A Validator node that proposes a block in the Polkadot network." .

ponto:nominates a owl:ObjectProperty ;
    rdfs:domain ponto:Nominator ;
    rdfs:range ponto:Validator ;
    rdfs:comment "A Nominator nominates a validator in the Polkadot network." .

ponto:validatesBlock a owl:ObjectProperty ;
    rdfs:domain ponto:Validator ;
    rdfs:range ponto:Transaction ;
    rdfs:comment "A Validator node that validates a block in the Polkadot network." .

ponto:validatesTransaction a owl:ObjectProperty ;
    rdfs:domain ponto:Validator ;
    rdfs:range ponto:Transaction ;
    rdfs:comment "A Validator node that validates a transaction." .

ponto:buildsBlock a owl:ObjectProperty ;
    rdfs:domain ponto:Collator ;
    rdfs:range ponto:Transaction ;
    rdfs:comment "A Collator node that builds a block for a specific parachain." .

ponto:collectsTransaction a owl:ObjectProperty ;
    rdfs:domain ponto:Collator ;
    rdfs:range ponto:Transaction ;
    rdfs:comment "A Collator node that collects transactions for a specific parachain." .

ponto:usesProofOfStake a owl:ObjectProperty ;
    rdfs:domain ponto:ProofOfStake ;
    rdfs:range ponto:Validator ;
    rdfs:comment "A Validator that participates in the ProofOfStake consensus mechanism." .
