@prefix ponto: <http://www.mobr.ai/ontologies/ponto#> .
@prefix owl: <http://www.w3.org/2002/07/owl#> .
@prefix rdf: <http://www.w3.org/1999/02/22-rdf-syntax-ns#> .
@prefix rdfs: <http://www.w3.org/2000/01/rdf-schema#> .

# oracle services in the Polkadot Ecosystem

ponto:Oracle a owl:Class ;
    rdfs:label "Oracle" ;
    rdfs:comment "Component that provides external data to smart contracts and decentralized applications (dApps) on the Polkadot network." ;
    rdfs:subClassOf ponto:Component .

ponto:DataFeed a owl:Class ;
    rdfs:label "Data Feed" ;
    rdfs:comment "A source of external data used by an oracle to provide data to a blockchain." ;
    rdfs:subClassOf ponto:Component .

ponto:Query a owl:Class ;
    rdfs:label "Query" ;
    rdfs:comment "A request for external data made by a smart contract or other component of a blockchain ecosystem." ;
    rdfs:subClassOf ponto:Component .
