@prefix ponto: <http://www.mobr.ai/ontologies/ponto#> .
@prefix owl: <http://www.w3.org/2002/07/owl#> .
@prefix rdf: <http://www.w3.org/1999/02/22-rdf-syntax-ns#> .
@prefix rdfs: <http://www.w3.org/2000/01/rdf-schema#> .

# wallet terminology
ponto:Wallet a owl:Class ;
    rdfs:label "Wallet" ;
    rdfs:comment "A program that allows one to store private keys and sign transactions on distributed ledgers" ;
    rdfs:subClassOf ponto:Component .

ponto:BrowserWallet a owl:Class ;
    rdfs:label "Browser Wallet" ;
    rdfs:comment "A wallet that runs in a web browser and can be accessed from any device." ;
    rdfs:subClassOf ponto:Wallet .

ponto:MobileWallet a owl:Class ;
    rdfs:label "Mobile Wallet" ;
    rdfs:comment "A wallet that runs on a mobile device and can be used to make payments on the go." ;
    rdfs:subClassOf ponto:Wallet .


# Polkadot wallet instances

ponto:Enkrypt a ponto:BrowserWallet ;
    rdfs:label "Enkrypt" ;
    rdfs:comment "A Polkadot wallet that supports multiple chains and allows users to manage their assets." .

ponto:PolkaGate a ponto:BrowserWallet ;
    rdfs:label "PolkaGate" ;
    rdfs:comment "A Polkadot wallet that supports multiple chains and allows users to manage their assets." .

ponto:SubWallet a ponto:BrowserWallet ;
    rdfs:label "SubWallet" ;
    rdfs:comment "A Polkadot wallet that supports Substrate-based chains and allows users to manage their assets." .

ponto:Talisman a ponto:BrowserWallet ;
    rdfs:label "Talisman" ;
    rdfs:comment "A Polkadot wallet that is designed to work with validator nodes and supports hardware wallets." .

ponto:FearlessWallet a ponto:MobileWallet ;
    rdfs:label "Fearless Wallet" ;
    rdfs:comment "A Polkadot wallet that is designed to be user-friendly and secure, with support for staking and governance." .

ponto:NovaWallet a ponto:MobileWallet ;
    rdfs:label "Nova Wallet" ;
    rdfs:comment "A Polkadot wallet that supports multiple chains and allows users to manage their assets." .

ponto:PolkaWallet a ponto:MobileWallet ;
    rdfs:label "PolkaWallet" ;
    rdfs:comment "A Polkadot wallet that supports multiple chains and allows users to manage their assets." .


#relationships
ponto:hasWallet rdfs:domain ponto:AccountHolder ;
    rdfs:range ponto:Wallet .
