@prefix ponto: <http://www.mobr.ai/ontologies/ponto#> .
@prefix owl: <http://www.w3.org/2002/07/owl#> .
@prefix rdf: <http://www.w3.org/1999/02/22-rdf-syntax-ns#> .
@prefix rdfs: <http://www.w3.org/2000/01/rdf-schema#> .
@prefix xsd: <http://www.w3.org/2001/XMLSchema#> .

# Assets and related subjects like account in the Polkadot Ecosystem

# assets
ponto:Asset a owl:Class ;
    rdfs:label "Asset" ;
    rdfs:comment "Representation of an asset on a distributed ledger." ;
    rdfs:subClassOf ponto:Component .

ponto:FungibleToken a owl:Class ;
    rdfs:label "Fungible Token" ;
    rdfs:comment "Divisible interchengable and non-unique unit of value that is used to represent assets on a distributed ledger." ;
    rdfs:subClassOf ponto:Asset .

ponto:NFT a owl:Class ;
    rdfs:label "Non-fungible Token" ;
    rdfs:comment "A non-fungible token is a token that does not hold the property of fungibility, which, in turn, means that it cannot be interchangeable and indistinguishable from other tokens. NFTs allow the tokenization of unique items and provide exclusive ownership for those tokens." ;
    rdfs:subClassOf ponto:Asset .

ponto:NativeToken a owl:Class ;
    rdfs:label "Native Token" ;
    rdfs:comment "The primary token used as the currency in a blockchain ecosystem, typically issued by the blockchain protocol itself." ;
    rdfs:subClassOf ponto:FungibleToken .

# account and account types

ponto:Account a owl:Class ;
    rdfs:label "Account" ;
    rdfs:comment "An address or a record on the blockchain that is used to store and manage cryptocurrency holdings or other types of assets." ;
    rdfs:subclasses ponto:LedgerRecord .

ponto:MultisigAccount a owl:Class ;
    rdfs:label "Multi-signature Account" ;
    rdfs:comment "A multisig is composed of one or more addresses and a threshold. The threshold defines how many signatories (participating addresses) need to agree on submitting an extrinsic for the call to be successful." ;
    rdfs:subclasses ponto:Account .

ponto:ProxyAccount a owl:Class ;
    rdfs:label "Proxy Account" ;
    rdfs:comment "Proxies are allowed to perform a limited amount of actions related to specific substrate pallets on behalf of another account." ;
    rdfs:subclasses ponto:Account .

ponto:ExternalAccount a owl:Class ;
    rdfs:label "External Account" ;
    rdfs:comment "An account that is controlled by an external system, such as an exchange or custodian." ;
    rdfs:subClassOf ponto:Account .

ponto:InjectedAccount a owl:Class ;
    rdfs:label "Injected Account" ;
    rdfs:comment "An account that is not directly managed by the Polkadot UI but can be accessed through it, such as accounts controlled by the Polkadot{.js} extension." ;
    rdfs:subClassOf ponto:Account .

ponto:NodeAccount a owl:Class ;
    rdfs:label "Node Account" ;
    rdfs:comment "An account that is used by a node to participate in block production or validation." ;
    rdfs:subClassOf ponto:Account .

ponto:SmartContract a owl:Class ;
    rdfs:label "Smart Contract" ;
    rdfs:comment "A self-executing contract that is stored on the blockchain and can interact with other contracts or accounts." ;
    rdfs:subClassOf ponto:Account .

ponto:CommunityQueue a owl:Class ;
    rdfs:label "Community Queue" ;
    rdfs:comment "The queue for proposals originating from individual accounts (i.e. not the Council) which are waiting to become referenda. Compare the External queue." ;
    rdfs:subClassOf ponto:Component .

ponto:ExternalQueue a owl:Class ;
    rdfs:label "External Queue" ;
    rdfs:comment "The queue for proposals originating with the Polkadot Council which are waiting to become referenda. Compare the Community queue." ;
    rdfs:subClassOf ponto:Component .

ponto:Crowdloan a owl:Class ;
    rdfs:label "Crowdloan" ;
    rdfs:comment "A mechanism for potential parachains to temporarily source tokens to win an auction for a parachain slot. Tokens gathered in this way are programmatically returned to the lender after the lease period is over or the crowdloan period ends." ;
    rdfs:subClassOf ponto:Component .

ponto:KeepAliveCheck a owl:Class ;
    rdfs:label "Keep-Alive Check" ;
    rdfs:comment "The keep-alive check is used to indicate whether or not a transfer can allow the sending account to be reduced to less than the existential deposit, causing it to be reaped." ;
    rdfs:subClassOf owl:Thing .

ponto:Teleport a owl:Class ;
    rdfs:label "Teleport" ;
    rdfs:comment "Send an asset from an account on one chain to an account on a different chain. This occurs by burning an amount on the sending chain and minting an equivalent amount on the destination chain." ;
    rdfs:subClassOf owl:Thing .

ponto:ReferenceCounter a owl:Class ;
    rdfs:label "RefCounter" ;
    rdfs:comment "Reference counters indicate the current state of an account. There are three types of reference counter: Sufficients, Consumers, and Providers." ;
    rdfs:subClassOf ponto:Component .

ponto:Sufficients a owl:Class ;
    rdfs:label "Sufficients" ;
    rdfs:comment "A reference counter to indicate if an account is self-sufficient and can exist by itself." ;
    rdfs:subClassOf ponto:ReferenceCounter .

ponto:Consumers a owl:Class ;
    rdfs:label "Consumers" ;
    rdfs:comment "A reference counter to indicate the number of other modules that currently depend on this account's existence. The account cannot be reaped until this is zero." ;
    rdfs:subClassOf ponto:ReferenceCounter .

ponto:Providers a owl:Class ;
    rdfs:label "Providers" ;
    rdfs:comment "A reference counter to indicate the number of other modules that allow this account to exist. The account may not be reaped until this (providers) and `sufficients` are both zero." ;
    rdfs:subClassOf ponto:ReferenceCounter .

ponto:LockType a owl:Class ;
    rdfs:label "Lock Type" ;
    rdfs:comment "Tokens may be locked. There are four types of lock: Staking, Democracy, Election, and Vesting." ;
    rdfs:subClassOf ponto:Component .

ponto:StakingLockType a owl:Class ;
    rdfs:label "Staking Lock Type" ;
    rdfs:comment "Probably the most common lock type. It applies when tokens are staked to nominate or validate. They can be bonded or unbonding." ;
    rdfs:subClassOf ponto:LockType .

ponto:DemocracyLockType a owl:Class ;
    rdfs:label "Democracy Lock Type" ;
    rdfs:comment "A lock type that applies when participating in democracy, usually through voting in referenda, either directly or through a delegation. See this page for more information on democracy locks." ;
    rdfs:subClassOf ponto:LockType .

ponto:ElectionLockType a owl:Class ;
    rdfs:label "Election Lock Type" ;
    rdfs:comment "A lock type that applies when voting for Council members." ;
    rdfs:subClassOf ponto:LockType .

ponto:VestingLockType a owl:Class ;
    rdfs:label "Vesting Lock Type" ;
    rdfs:comment "A lock type that can be applied by the sender of tokens through a 'vested transfer'. These tokens are received locked, and unlock over a period of time, usually in small increments. Vesting tokens unlock based on a vesting schedule and are considered lazy payouts, but they can be used for any other action that introduces a lock." ;
    rdfs:subClassOf ponto:LockType .

# literals
ponto:Balance a owl:Class ;
    rdfs:label "Balance" ;
    rdfs:comment "Token balance controlled by an account holder" .
    rdfs:subClassOf ponto:Component .

ponto:ReservedBalance a owl:Class ;
    rdfs:label "Reserved Balance" ;
    rdfs:comment "Certain actions require reserving transferable tokens to use space in the chain state. These tokens act as a deposit that is set aside for an operation and still belongs to the account holder but cannot be used for other operations. The tokens are reserved for as long as the reason exists. Once the reason is removed, the balance becomes transferable once again." ;
    rdfs:subClassOf ponto:Balance .

ponto:ReservationReason a owl:Class ;
    rdfs:label "Reservation Reason" ;
    rdfs:comment "Certain actions require reserving transferable tokens to use space in the chain state. These tokens act as a deposit that is set aside for an operation and still belongs to the account holder but cannot be used for other operations. The tokens are reserved for as long as the reason exists. Once the reason is removed, the balance becomes transferable once again." ;
    rdfs:subClassOf ponto:Component .

ponto:LockedBalance a owl:Class ;
    rdfs:label "Locked Balance" ;
    rdfs:comment "When tokens are used to serve their utility purpose on the chain, they are locked. The account holder still controls locked tokens. They cannot be transferred, but they can be used for multiple operations at the same time. For example, the same locked tokens can be used to nominate validators and vote in democracy." ;
    rdfs:subClassOf ponto:Balance .

ponto:TransferableBalance a owl:Class ;
    rdfs:label "Transferable Balance" ;
    rdfs:comment "Transferable tokens are fully available. These tokens are the ones that can be transferred, used to pay transaction fees, and become locked or reserved for other purposes. " ;
    rdfs:subClassOf ponto:Balance .

# relationships
ponto:hasLockType a owl:ObjectProperty ;
        rdfs:domain ponto:LockedBalance ;
        rdfs:range ponto:LockType .

ponto:hasAddress a owl:DatatypeProperty ;
    rdfs:comment "An account has an address." ;
    rdfs:domain ponto:Account ;
    rdfs:range xsd:string .

ponto:hasRefCountValue a owl:DatatypeProperty ;
    rdfs:domain ponto:RefCounter ;
    rdfs:range xsd:integer .

ponto:hasSufficients a owl:ObjectProperty ;
    rdfs:domain ponto:Account ;
    rdfs:range ponto:Sufficients .

ponto:hasConsumers a owl:ObjectProperty ;
    rdfs:domain ponto:Account ;
    rdfs:range ponto:Consumers .

ponto:hasProviders a owl:ObjectProperty ;
    rdfs:domain ponto:Account ;
    rdfs:range ponto:Providers .

ponto:bonding a rdf:Property ;
    rdfs:comment "A process by which tokens can be 'frozen' in exchange for some other benefit. For example, staking is a form of bonding for which you receive rewards in exchange for securing the network. You can also bond tokens in exchange for a parachain slot." ;
    rdfs:domain ponto:Asset ;
    rdfs:range xsd:decimal .

# a wallet has one or more accounts
ponto:hasAccount a owl:ObjectProperty ;
    rdfs:domain ponto:Wallet ;
    rdfs:range ponto:Account .

ponto:hasAccount owl:inverseOf ponto:isAccountOf .

ponto:accountCreated a owl:DatatypeProperty ;
    rdfs:comment "The timestamp when the account was created." ;
    rdfs:domain ponto:Account ;
    rdfs:range xsd:dateTimeStamp .

# an account has one or more types of tokens
ponto:hasToken a owl:ObjectProperty ;
    rdfs:domain ponto:Account ;
    rdfs:range ponto:Asset .

# balance of a token
ponto:hasBalanceValue a owl:DatatypeProperty ;
    rdfs:domain ponto:Balance ;
    rdfs:range xsd:decimal .

ponto:hasTransferableBalance a owl:ObjectProperty ;
    rdfs:domain ponto:FungibleToken ;
    rdfs:range ponto:TransferableBalance .

ponto:hasReservedBalance a owl:ObjectProperty ;
    rdfs:domain ponto:FungibleToken ;
    rdfs:range ponto:ReservedBalance .

ponto:reservedFor a owl:ObjectProperty ;
    rdfs:comment "Tokens can be reserved for various reasons that use space in the chain state. Unlike locks, reserves do stack. So, each new action that requires a deposit reserves the necessary amount added to any previous reserves that might exist." ;
    rdfs:domain ponto:ReservedBalance ;
    rdfs:range ponto:ReservationReason .

ponto:hasReasonDescription a owl:DatatypeProperty ;
    rdfs:domain ponto:ReservationReason ;
    rdfs:range xsd:string .

ponto:makesReservation a owl:ObjectProperty ;
    rdfs:domain ponto:LedgerRecord ;
    rdfs:range ponto:ReservedBalance .

ponto:hasLockedBalance a owl:ObjectProperty ;
    rdfs:domain ponto:FungibleToken ;
    rdfs:range ponto:LockedBalance .

ponto:hasSymbol a owl:DatatypeProperty ;
    rdfs:domain ponto:FungibleToken ;
    rdfs:range xsd:string .

ponto:hasName a owl:DatatypeProperty ;
    rdfs:domain ponto:FungibleToken ;
    rdfs:range xsd:string .

# native tokens
ponto:DOT a owl:Class ;
    rdfs:label "DOT" ;
    rdfs:comment "The native token for Polkadot. DOT serves three purposes: network governance (allowing them to vote on-chain upgrades and other exceptional events), general operation (rewarding good actors and punishing bad actors), and bonding (adding new parachains by 'freezing' DOT while they are connected the Relay Chain)." ;
    rdfs:subClassOf ponto:NativeToken .

ponto:KSM a owl:Class ;
    rdfs:label "KSM" ;
    rdfs:comment "The native token for the Kusama network" ;
    rdfs:subClassOf ponto:NativeToken .
